add assoc checked arg bridge reductions

rocq/theories/TypeSystem/AssocCheckedBridgeReductionFacts.v
@@ -1,5 +1,18 @@
 From Facet.TypeSystem Require Import
-  Lifetime Types Syntax Program TypingRules AssocCompatibility.
+  Lifetime Types Syntax Program TypingRules CheckerBase AssocCompatibility.
+From Stdlib Require Import List.
+
+Definition ty_compatible_assoc_checked_reduces_to_plain
+    (env : global_env) (Ω : outlives_ctx) : Prop :=
+  forall actual expected,
+    ty_compatible_assoc_checked env Ω actual expected ->
+    ty_compatible Ω actual expected.
+
+Definition ty_compatible_assoc_checked_reduces_to_bool
+    (env : global_env) (Ω : outlives_ctx) : Prop :=
+  forall actual expected,
+    ty_compatible_assoc_checked env Ω actual expected ->
+    ty_compatible_b Ω actual expected = true.
 
 Definition ty_compatible_assoc_checked_reduces_to_assoc
     (env : global_env) (Ω : outlives_ctx) : Prop :=
@@ -17,4 +30,35 @@ Proof.
   induction Hargs.
   - constructor.
   - econstructor; eauto.
+Qed.
+
+Lemma typed_args_assoc_checked_reduces_to_plain :
+  forall env fenv Ω n Γ args ps Γ',
+    ty_compatible_assoc_checked_reduces_to_plain env Ω ->
+    typed_args_assoc_checked env fenv Ω n Γ args ps Γ' ->
+    typed_args fenv Ω n Γ args ps Γ'.
+Proof.
+  intros env fenv Ω n Γ args ps Γ' Hcompat Hargs.
+  induction Hargs.
+  - constructor.
+  - econstructor; eauto.
+Qed.
+
+Lemma typed_args_assoc_checked_reduces_to_bool :
+  forall env fenv Ω n Γ args ps Γ',
+    ty_compatible_assoc_checked_reduces_to_bool env Ω ->
+    typed_args_assoc_checked env fenv Ω n Γ args ps Γ' ->
+    Forall2
+      (fun e p =>
+        exists actual Γin Γout,
+          typed fenv Ω n Γin e actual Γout /\
+          ty_compatible_b Ω actual (param_ty p) = true)
+      args ps.
+Proof.
+  intros env fenv Ω n Γ args ps Γ' Hcompat Hargs.
+  induction Hargs.
+  - constructor.
+  - constructor.
+    + exists T_e, Γ, Γ1. split; eauto.
+    + exact IHHargs.
 Qed.
