rocq/theories/TypeSystem/AssocStructFieldBridgeReductionFacts.v
@@ -1,14 +1,8 @@
 From Facet.TypeSystem Require Import
   Lifetime Types Syntax Program TypingRules AssocCompatibility
-  AssocStructFieldTypingFacts.
+  AssocCheckedBridgeReductionFacts AssocStructFieldTypingFacts.
 From Stdlib Require Import List String.
 Import ListNotations.
-
-Definition ty_compatible_assoc_checked_reduces_to_plain
-    (env : global_env) (Ω : outlives_ctx) : Prop :=
-  forall actual expected,
-    ty_compatible_assoc_checked env Ω actual expected ->
-    ty_compatible Ω actual expected.
 
 Lemma typed_struct_fields_assoc_checked_reduces_to_struct_fields :
   forall env fenv Ω n lts args Γ fields defs Γ',
